proving more

dev/lf/dot_top_bot_mut2.v
@@ -1995,82 +1995,82 @@ Proof.
 Qed.
 
 Lemma precise_to_general:
-  (forall m1 m2 G t T,
-     ty_trm m1 m2 G t T ->
+  (forall m1 m2 G S t T,
+     ty_trm m1 m2 G S t T ->
      m1 = ty_precise ->
      m2 = sub_general ->
-     ty_trm ty_general sub_general G t T) /\
-  (forall m1 m2 G S U,
-     subtyp m1 m2 G S U ->
+     ty_trm ty_general sub_general G S t T) /\
+  (forall m1 m2 G S V U,
+     subtyp m1 m2 G S V U ->
      m1 = ty_precise ->
      m2 = sub_general ->
-     subtyp ty_general sub_general G S U).
+     subtyp ty_general sub_general G S V U).
 Proof.
   apply ts_mutind; intros; subst; eauto.
 Qed.
 
-Lemma precise_to_general_typing: forall G t T,
-  ty_trm ty_precise sub_general G t T ->
-  ty_trm ty_general sub_general G t T.
+Lemma precise_to_general_typing: forall G S t T,
+  ty_trm ty_precise sub_general G S t T ->
+  ty_trm ty_general sub_general G S t T.
 Proof.
   intros. apply* precise_to_general.
 Qed.
 
 Lemma tight_to_general:
-  (forall m1 m2 G t T,
-     ty_trm m1 m2 G t T ->
+  (forall m1 m2 G S t T,
+     ty_trm m1 m2 G S t T ->
      m1 = ty_general ->
      m2 = sub_tight ->
-     ty_trm ty_general sub_general G t T) /\
-  (forall m1 m2 G S U,
-     subtyp m1 m2 G S U ->
+     ty_trm ty_general sub_general G S t T) /\
+  (forall m1 m2 G S V U,
+     subtyp m1 m2 G S V U ->
      m1 = ty_general ->
      m2 = sub_tight ->
-     subtyp ty_general sub_general G S U).
+     subtyp ty_general sub_general G S V U).
 Proof.
   apply ts_mutind; intros; subst; eauto.
   - apply precise_to_general in t; eauto.
   - apply precise_to_general in t; eauto.
 Qed.
 
-Lemma tight_to_general_typing: forall G t T,
-  ty_trm ty_general sub_tight G t T ->
-  ty_trm ty_general sub_general G t T.
+Lemma tight_to_general_typing: forall G S t T,
+  ty_trm ty_general sub_tight G S t T ->
+  ty_trm ty_general sub_general G S t T.
 Proof.
   intros. apply* tight_to_general.
 Qed.
 
-Lemma tight_to_general_subtyping: forall G S U,
-  subtyp ty_general sub_tight G S U ->
-  subtyp ty_general sub_general G S U.
+Lemma tight_to_general_subtyping: forall G S V U,
+  subtyp ty_general sub_tight G S V U ->
+  subtyp ty_general sub_general G S V U.
 Proof.
   intros. apply* tight_to_general.
 Qed.
 
 Lemma precise_to_tight:
-  (forall m1 m2 G t T,
-     ty_trm m1 m2 G t T ->
+  (forall m1 m2 G S t T,
+     ty_trm m1 m2 G S t T ->
      m1 = ty_precise ->
      m2 = sub_general ->
-     ty_trm ty_general sub_tight G t T) /\
-  (forall m1 m2 G S U,
-     subtyp m1 m2 G S U ->
+     ty_trm ty_general sub_tight G S t T) /\
+  (forall m1 m2 G S V U,
+     subtyp m1 m2 G S V U ->
      m1 = ty_precise ->
      m2 = sub_general ->
-     subtyp ty_general sub_tight G S U).
+     subtyp ty_general sub_tight G S V U).
 Proof.
   apply ts_mutind; intros; subst; eauto; inversion H0.
 Qed.
 
-Lemma precise_to_tight_typing: forall G t T,
-  ty_trm ty_precise sub_general G t T ->
-  ty_trm ty_general sub_tight G t T.
+Lemma precise_to_tight_typing: forall G S t T,
+  ty_trm ty_precise sub_general G S t T ->
+  ty_trm ty_general sub_tight G S t T.
 Proof.
   intros. apply* precise_to_tight.
 Qed.
 
-Lemma stack_binds_to_ctx_binds: forall G s x v,
-  wf_stack G s -> binds x v s -> exists S, binds x S G.
+Lemma stack_binds_to_ctx_binds: forall G S s x v,
+  wf_stack G S s -> binds x v s -> exists V, binds x V G.
 Proof.
   introv Hwf Bis.
   remember Hwf as Hwf'. clear HeqHwf'.
@@ -2083,8 +2083,8 @@ Proof.
   assumption.
 Qed.
 
-Lemma ctx_binds_to_stack_binds: forall G s x T,
-  wf_stack G s -> binds x T G -> exists v, binds x v s.
+Lemma ctx_binds_to_stack_binds: forall G S s x T,
+  wf_stack G S s -> binds x T G -> exists v, binds x v s.
 Proof.
   introv Hwf Bi.
   remember Hwf as Hwf'. clear HeqHwf'.
@@ -2096,35 +2096,37 @@ Proof.
   assumption.
 Qed.
 
-Lemma record_type_new: forall G s x T ds,
-  wf_stack G s ->
+Lemma record_type_new: forall G S s x T ds,
+  wf_stack G S s ->
   binds x (val_new T ds) s ->
   record_type (open_typ x T).
 Proof.
   introv Hwf Bis.
-  destruct (stack_binds_to_ctx_binds Hwf Bis) as [S Bi].
-  destruct (corresponding_types Hwf Bi) as [Hlambda | Hnew].
-  destruct Hlambda as [? [? [? [Bis' ?]]]].
-  unfold binds in Bis'. unfold binds in Bis. rewrite Bis' in Bis. inversions Bis.
-  destruct Hnew as [? [? [Bis' [? ?]]]]. subst.
-  unfold binds in Bis'. unfold binds in Bis. rewrite Bis' in Bis. inversions Bis.
-  apply record_new_typing in H.
-  apply open_record_type. assumption.
+  destruct (stack_binds_to_ctx_binds Hwf Bis) as [V Bi].
+  destruct (corresponding_types_ctx Hwf Bi) as [[Hlambda | Hnew] | Hloc].
+  - destruct Hlambda as [? [? [? [Bis' ?]]]].
+    unfold binds in Bis'. unfold binds in Bis. rewrite Bis' in Bis. inversions Bis.
+  - destruct Hnew as [? [? [Bis' [? ?]]]]. subst.
+    unfold binds in Bis'. unfold binds in Bis. rewrite Bis' in Bis. inversions Bis.
+    apply record_new_typing in H.
+    apply open_record_type. assumption.
+  - destruct Hloc as [? [? [Bil [?]]]].
+    unfold binds in *. rewrite Bil in Bis. inversion Bis.
 Qed.
 
 (* ###################################################################### *)
 (** ** Narrowing *)
 
-Definition subenv(G1 G2: ctx) :=
+Definition subenv(G1 G2: ctx) (S: sigma) :=
   forall x T2, binds x T2 G2 ->
     binds x T2 G1 \/
     exists T1,
-      binds x T1 G1 /\ subtyp ty_general sub_general G1 T1 T2.
+      binds x T1 G1 /\ subtyp ty_general sub_general G1 S T1 T2.
 
-Lemma subenv_push: forall G G' x T,
-  subenv G' G ->
+Lemma subenv_push: forall G G' S x T,
+  subenv G' G S ->
   ok (G' & x ~ T) ->
-  subenv (G' & x ~ T) (G & x ~ T).
+  subenv (G' & x ~ T) (G & x ~ T) S.
 Proof.
   intros.
   unfold subenv. intros xb Tb Bi. apply binds_push_inv in Bi.
@@ -2138,79 +2140,80 @@ Proof.
       exists T'. split. eauto. apply weaken_subtyp. assumption. eauto.
 Qed.
 
-Lemma subenv_last: forall G x S U,
-  subtyp ty_general sub_general G S U ->
-  ok (G & x ~ S) ->
-  subenv (G & x ~ S) (G & x ~ U).
+Lemma subenv_last: forall G S x V U,
+  subtyp ty_general sub_general G S V U ->
+  ok (G & x ~ V) ->
+  subenv (G & x ~ V) (G & x ~ U) S.
 Proof.
   intros. unfold subenv. intros y T Bi.
   apply binds_push_inv in Bi. destruct Bi as [Bi | Bi].
-  - destruct Bi. subst. right. exists S. split; eauto.
+  - destruct Bi. subst. right. exists V. split; eauto.
     apply weaken_subtyp; eauto.
   - destruct Bi. left. eauto.
 Qed.
 
+
 Lemma narrow_rules:
-  (forall m1 m2 G t T, ty_trm m1 m2 G t T -> forall G',
+  (forall m1 m2 G S t T, ty_trm m1 m2 G S t T -> forall G',
     m1 = ty_general ->
     m2 = sub_general ->
     ok G' ->
-    subenv G' G ->
-    ty_trm m1 m2 G' t T)
-/\ (forall G d D, ty_def G d D -> forall G',
+    subenv G' G S ->
+    ty_trm m1 m2 G' S t T)
+/\ (forall G S d D, ty_def G S d D -> forall G',
     ok G' ->
-    subenv G' G ->
-    ty_def G' d D)
-/\ (forall G ds T, ty_defs G ds T -> forall G',
+    subenv G' G S ->
+    ty_def G' S d D)
+/\ (forall G S ds T, ty_defs G S ds T -> forall G',
     ok G' ->
-    subenv G' G ->
-    ty_defs G' ds T)
-/\ (forall m1 m2 G S U, subtyp m1 m2 G S U -> forall G',
+    subenv G' G S ->
+    ty_defs G' S ds T)
+/\ (forall m1 m2 G S V U, subtyp m1 m2 G S V U -> forall G',
     m1 = ty_general ->
     m2 = sub_general ->
     ok G' ->
-    subenv G' G ->
-    subtyp m1 m2 G' S U).
+    subenv G' G S ->
+    subtyp m1 m2 G' S V U).
 Proof.
   apply rules_mutind; intros; eauto.
   - (* ty_var *)
     subst. unfold subenv in H2. specialize (H2 x T b).
     destruct H2.
-    + eauto.
+    + auto.
     + destruct H as [T' [Bi Hsub]].
       eapply ty_sub; eauto.
   - (* ty_all_intro *)
     subst.
-    apply_fresh ty_all_intro as y; eauto.
-    eapply H; eauto. apply subenv_push; eauto.
+    apply_fresh ty_all_intro as y; auto.
+    apply H; auto. apply subenv_push; auto.
   - (* ty_new_intro *)
     subst.
-    apply_fresh ty_new_intro as y; eauto.
-    apply H; eauto. apply subenv_push; eauto.
+    apply_fresh ty_new_intro as y; auto.
+    apply H; auto. apply subenv_push; auto.
   - (* ty_let *)
     subst.
-    apply_fresh ty_let as y; eauto.
-    apply H0 with (x:=y); eauto. apply subenv_push; eauto.
+    apply_fresh ty_let as y; auto.
+    apply H0 with (x:=y); auto. apply subenv_push; auto.
   - inversion H1 (* sub_tight *).
   - inversion H1 (* sub_tight *).
   - (* subtyp_all *)
     subst.
-    apply_fresh subtyp_all as y; eauto.
-    apply H0; eauto. apply subenv_push; eauto.
+    apply_fresh subtyp_all as y; auto.
+    apply H0; auto. apply subenv_push; auto.
 Qed.
 
-Lemma narrow_typing: forall G G' t T,
-  ty_trm ty_general sub_general G t T ->
-  subenv G' G -> ok G' ->
-  ty_trm ty_general sub_general G' t T.
+Lemma narrow_typing: forall G G' S t T,
+  ty_trm ty_general sub_general G S t T ->
+  subenv G' G S -> ok G' ->
+  ty_trm ty_general sub_general G' S t T.
 Proof.
   intros. apply* narrow_rules.
 Qed.
 
-Lemma narrow_subtyping: forall G G' S U,
-  subtyp ty_general sub_general G S U ->
-  subenv G' G -> ok G' ->
-  subtyp ty_general sub_general G' S U.
+Lemma narrow_subtyping: forall G G' S V U,
+  subtyp ty_general sub_general G S V U ->
+  subenv G' G S -> ok G' ->
+  subtyp ty_general sub_general G' S V U.
 Proof.
   intros. apply* narrow_rules.
 Qed.
@@ -2218,88 +2221,90 @@ Qed.
 (* ###################################################################### *)
 (** * Has member *)
 
-Inductive has_member: ctx -> var -> typ -> typ_label -> typ -> typ -> Prop :=
-| has_any : forall G x T A S U,
-  ty_trm ty_general sub_tight G (trm_var (avar_f x)) T ->
-  has_member_rules G x T A S U ->
-  has_member G x T A S U
-with has_member_rules: ctx -> var -> typ -> typ_label -> typ -> typ -> Prop :=
-| has_refl : forall G x A S U,
-  has_member_rules G x (typ_rcd (dec_typ A S U)) A S U
-| has_and1 : forall G x T1 T2 A S U,
-  has_member G x T1 A S U ->
-  has_member_rules G x (typ_and T1 T2) A S U
-| has_and2 : forall G x T1 T2 A S U,
-  has_member G x T2 A S U ->
-  has_member_rules G x (typ_and T1 T2) A S U
-| has_bnd : forall G x T A S U,
-  has_member G x (open_typ x T) A S U ->
-  has_member_rules G x (typ_bnd T) A S U
-| has_sel : forall G x y B T' A S U,
-  ty_trm ty_precise sub_general G (trm_var (avar_f y)) (typ_rcd (dec_typ B T' T')) ->
-  has_member G x T' A S U ->
-  has_member_rules G x (typ_sel (avar_f y) B) A S U
-| has_bot  : forall G x A S U,
-  has_member_rules G x typ_bot A S U
-.
+Inductive has_member: ctx -> sigma -> var -> typ -> typ_label -> typ -> typ -> Prop :=
+| has_any : forall G S x T A V U,
+  ty_trm ty_general sub_tight G S (trm_var (avar_f x)) T ->
+  has_member_rules G S x T A V U ->
+  has_member G S x T A V U
+with has_member_rules: ctx -> sigma ->var -> typ -> typ_label -> typ -> typ -> Prop :=
+| has_refl : forall G S x A V U,
+  has_member_rules G S x (typ_rcd (dec_typ A V U)) A V U
+| has_and1 : forall G S x T1 T2 A V U,
+  has_member G S x T1 A V U ->
+  has_member_rules G S x (typ_and T1 T2) A V U
+| has_and2 : forall G S x T1 T2 A V U,
+  has_member G S x T2 A V U ->
+  has_member_rules G S x (typ_and T1 T2) A V U
+| has_bnd : forall G S x T A V U,
+  has_member G S x (open_typ x T) A V U ->
+  has_member_rules G S x (typ_bnd T) A V U
+| has_sel : forall G S x y B T' A V U,
+  ty_trm ty_precise sub_general G S (trm_var (avar_f y)) (typ_rcd (dec_typ B T' T')) ->
+  has_member G S x T' A V U ->
+  has_member_rules G S x (typ_sel (avar_f y) B) A V U
+| has_bot  : forall G S x A V U,
+  has_member_rules G S x typ_bot A V U.
+
 
 Scheme has_mut := Induction for has_member Sort Prop
 with hasr_mut := Induction for has_member_rules Sort Prop.
 Combined Scheme has_mutind from has_mut, hasr_mut.
 
-Lemma has_member_rules_inv: forall G x T A S U, has_member_rules G x T A S U ->
-  (T = typ_rcd (dec_typ A S U)) \/
+Lemma has_member_rules_inv: forall G S x T A V U, has_member_rules G S x T A V U ->
+  (T = typ_rcd (dec_typ A V U)) \/
   (exists T1 T2, T = typ_and T1 T2 /\
-    (has_member G x T1 A S U \/
-     has_member G x T2 A S U)) \/
+    (has_member G S x T1 A V U \/
+     has_member G S x T2 A V U)) \/
   (exists T', T = typ_bnd T' /\
-    has_member G x (open_typ x T') A S U) \/
+    has_member G S x (open_typ x T') A V U) \/
   (exists y B T', T = typ_sel (avar_f y) B /\
-    ty_trm ty_precise sub_general G (trm_var (avar_f y)) (typ_rcd (dec_typ B T' T')) /\
-    has_member G x T' A S U) \/
+    ty_trm ty_precise sub_general G S (trm_var (avar_f y)) (typ_rcd (dec_typ B T' T')) /\
+    has_member G S x T' A V U) \/
   (T = typ_bot).
 Proof.
   intros. inversion H; subst.
-  - left. eauto.
-  - right. left. exists T1 T2. eauto.
-  - right. left. exists T1 T2. eauto.
-  - right. right. left. exists T0. eauto.
-  - right. right. right. left. exists y B T'. eauto.
+  - left. auto.
+  - right. left. exists T1 T2. auto.
+  - right. left. exists T1 T2. auto.
+  - right. right. left. exists T0. auto.
+  - right. right. right. left. exists y B T'. auto.
   - right. right. right. right. reflexivity.
 Qed.
 
-Lemma has_member_inv: forall G x T A S U, has_member G x T A S U ->
-  (T = typ_rcd (dec_typ A S U)) \/
+Lemma has_member_inv: forall G S x T A V U, has_member G S x T A V U ->
+  (T = typ_rcd (dec_typ A V U)) \/
   (exists T1 T2, T = typ_and T1 T2 /\
-    (has_member G x T1 A S U \/
-     has_member G x T2 A S U)) \/
+    (has_member G S x T1 A V U \/
+     has_member G S x T2 A V U)) \/
   (exists T', T = typ_bnd T' /\
-    has_member G x (open_typ x T') A S U) \/
+    has_member G S x (open_typ x T') A V U) \/
   (exists y B T', T = typ_sel (avar_f y) B /\
-    ty_trm ty_precise sub_general G (trm_var (avar_f y)) (typ_rcd (dec_typ B T' T')) /\
-    has_member G x T' A S U) \/
+    ty_trm ty_precise sub_general G S (trm_var (avar_f y)) (typ_rcd (dec_typ B T' T')) /\
+    has_member G S x T' A V U) \/
   (T = typ_bot).
 Proof.
   intros. inversion H; subst. apply has_member_rules_inv in H1. apply H1.
 Qed.
 
-Lemma val_new_typing: forall G s x T ds,
-  wf_stack G s ->
+Lemma val_new_typing: forall G S s x T ds,
+  wf_stack G S s ->
   binds x (val_new T ds) s ->
-  ty_trm ty_precise sub_general G (trm_val (val_new T ds)) (typ_bnd T).
+  ty_trm ty_precise sub_general G S (trm_val (val_new T ds)) (typ_bnd T).
 Proof.
   introv Hwf Bis.
   assert (exists T, binds x T G) as Bi. {
     eapply stack_binds_to_ctx_binds; eauto.
   }
   destruct Bi as [T0 Bi].
-  destruct (corresponding_types Hwf Bi).
-  - destruct H as [S [U [t [Bis' [Ht EqT]]]]].
+  destruct (corresponding_types_ctx Hwf Bi) as [[Hnew | Hlambda] | Hloc].
+  - destruct Hnew as [V [U [t [Bis' [Ht EqT]]]]].
     false.
-  - destruct H as [T' [ds' [Bis' [Ht EqT]]]]. subst.
+  - destruct Hlambda as [T' [ds' [Bis' [Ht EqT]]]]. subst.
     unfold binds in Bis. unfold binds in Bis'. rewrite Bis' in Bis.
     inversion Bis. subst.
     assumption.
+  - destruct Hloc as [V [l [Bi' [Htyp]]]].
+    false.
 Qed.
 
 
@@ -2317,33 +2322,33 @@ Proof.
 Qed.
 
 Lemma has_member_rcd_typ_sub_mut:
-  (forall G x T A S U,
-    has_member G x T A S U ->
+  (forall G S x T A V U,
+    has_member G S x T A V U ->
     record_type T ->
-    record_sub T (typ_rcd (dec_typ A S U))) /\
-  (forall G x T A S U,
-    has_member_rules G x T A S U ->
+    record_sub T (typ_rcd (dec_typ A V U))) /\
+  (forall G S x T A V U,
+    has_member_rules G S x T A V U ->
     record_type T ->
-    record_sub T (typ_rcd (dec_typ A S U))).
+    record_sub T (typ_rcd (dec_typ A V U))).
 Proof.
   apply has_mutind; intros.
   - apply H; eauto.
   - apply rs_refl.
   - inversion H0; subst. inversion H1; subst. apply rs_drop.
-    apply H; eauto.
+    apply H; auto.
     exists ls. assumption.
   - inversion H0; subst. inversion H1; subst. inversion h; subst. inversion H3; subst.
-    eapply rs_dropl. eapply rs_refl.
+    eapply rs_dropl. apply rs_refl.
   - inversion H0. inversion H1.
   - inversion H0. inversion H1.
   - destruct H as [ls H]. inversion H.
 Qed.
 
-Lemma has_member_tightness: forall G s x T ds A S U,
-  wf_stack G s ->
+Lemma has_member_tightness: forall G S s x T ds A V U,
+  wf_stack G S s ->
   binds x (val_new T ds) s ->
-  has_member G x (typ_bnd T) A S U ->
-  S = U.
+  has_member G S x (typ_bnd T) A V U ->
+  V = U.
 Proof.
   introv Hwf Bis Hmem.
   assert (record_type T) as Htype. {
@@ -2352,24 +2357,24 @@ Proof.
   assert (record_type (open_typ x T)) as Htypex. {
     apply open_record_type. assumption.
   }
-  assert (has_member G x (open_typ x T) A S U) as Hmemx. {
+  assert (has_member G S x (open_typ x T) A V U) as Hmemx. {
     inversion Hmem; subst. inversion H0; subst. assumption.
   }
-  assert (record_sub (open_typ x T) (typ_rcd (dec_typ A S U))) as Hsub. {
+  assert (record_sub (open_typ x T) (typ_rcd (dec_typ A V U))) as Hsub. {
     destruct has_member_rcd_typ_sub_mut as [HL _].
     eapply HL; eauto.
   }
-  eapply rcd_typ_eq_bounds. eapply Htypex. eapply Hsub.
+  eapply rcd_typ_eq_bounds. apply Htypex. apply Hsub.
 Qed.
 
-Lemma has_member_covariance: forall G s T1 T2 x A S2 U2,
-  wf_stack G s ->
-  subtyp ty_general sub_tight G T1 T2 ->
-  ty_trm ty_general sub_tight G (trm_var (avar_f x)) T1 ->
-  has_member G x T2 A S2 U2 ->
-  exists S1 U1, has_member G x T1 A S1 U1 /\
-                subtyp ty_general sub_tight G S2 S1 /\
-                subtyp ty_general sub_tight G U1 U2.
+Lemma has_member_covariance: forall G S s T1 T2 x A S2 U2,
+  wf_stack G S s ->
+  subtyp ty_general sub_tight G S T1 T2 ->
+  ty_trm ty_general sub_tight G S (trm_var (avar_f x)) T1 ->
+  has_member G S x T2 A S2 U2 ->
+  exists S1 U1, has_member G S x T1 A S1 U1 /\
+                subtyp ty_general sub_tight G S S2 S1 /\
+                subtyp ty_general sub_tight G S U1 U2.
 Proof.
   introv Hwf Hsub Hty Hmem.
   generalize dependent U2.
@@ -2384,7 +2389,7 @@ Proof.
   - (* refl *)
     exists S2 U2. eauto.
   - (* trans *)
-    assert (ty_trm ty_general sub_tight G (trm_var (avar_f x)) T) as HS. {
+    assert (ty_trm ty_general sub_tight G S (trm_var (avar_f x)) T) as HS. {
       eapply ty_sub. intros Hp. subst. eexists; eauto.
       eapply Hty.
       eassumption.
@@ -2445,29 +2450,32 @@ Proof.
     inversion Hmem; subst. inversion H2; subst.
 Qed.
 
-Lemma has_member_monotonicity: forall G s x T0 ds T A S U,
-  wf_stack G s ->
+Lemma has_member_monotonicity: forall G S s x T0 ds T A V U,
+  wf_stack G S s ->
   binds x (val_new T0 ds) s ->
-  has_member G x T A S U ->
-  exists T1, has_member G x (typ_bnd T0) A T1 T1 /\
-             subtyp ty_general sub_tight G S T1 /\
-             subtyp ty_general sub_tight G T1 U.
+  has_member G S x T A V U ->
+  exists T1, has_member G S x (typ_bnd T0) A T1 T1 /\
+             subtyp ty_general sub_tight G S V T1 /\
+             subtyp ty_general sub_tight G S T1 U.
 Proof.
   introv Hwf Bis Hmem. inversion Hmem; subst.
-  generalize dependent U. generalize dependent S.
+  generalize dependent U. generalize dependent V.
   dependent induction H; intros.
   - (* var *)
-    destruct (corresponding_types Hwf H).
-    destruct H1 as [S0 [U0 [t [Bis' _]]]]. unfold binds in Bis'. unfold binds in Bis. rewrite Bis' in Bis. inversion Bis.
-    destruct H1 as [S0 [ds0 [Bis' [Hty Heq]]]]. unfold binds in Bis'. unfold binds in Bis. rewrite Bis in Bis'. inversions Bis'.
-    assert (S = U). {
-      eapply has_member_tightness. eassumption. eassumption.
-      eapply has_any.
-      eapply ty_var. eassumption.
-      eassumption.
-    }
-    subst.
-    exists U. eauto.
+    destruct (corresponding_types_ctx Hwf H). destruct H1 as [Hlam | Hnew].
+    * destruct Hlam as [S0 [U0 [t [Bis' _]]]].
+      unfold binds in Bis'. unfold binds in Bis. rewrite Bis' in Bis. inversion Bis.
+    * destruct Hnew as [S0 [ds0 [Bis' [Hty Heq]]]]. unfold binds in Bis'. unfold binds in Bis.
+      rewrite Bis in Bis'. inversions Bis'.
+      assert (V = U). {
+        eapply has_member_tightness. eassumption. eassumption.
+        eapply has_any.
+        eapply ty_var. eassumption.
+        eassumption.
+      }
+      subst. exists U. eauto. 
+    * destruct H1 as [V0 [l [Bi' [Htyp]]]].
+      unfold binds in Bis. unfold binds in Bi'. rewrite Bi' in Bis. inversion Bis.
   - (* rec_intro *)
     apply has_member_inv in Hmem.
     repeat destruct Hmem as [Hmem|Hmem].
@@ -2476,7 +2484,7 @@ Proof.
     + destruct Hmem as [T1' [Heq _]]. inversions Heq.
       apply IHty_trm; eauto.
       inversions H0. assumption.
-      inversions H0. inversions H4. assumption.
+      inversions H0. inversions H5. assumption.
     + destruct Hmem as [y [B [T' [Heq [Htyb Hmem]]]]]. inversion Heq.
     + inversion Hmem.
   - (* rec_elim *)
@@ -2488,7 +2496,7 @@ Proof.
     repeat destruct Hmem as [Hmem|Hmem].
     + inversion Hmem.
     + destruct Hmem as [T1' [T2' [Heq [Hmem | Hmem]]]];
-      inversions Heq; inversions H1; inversions H9.
+      inversions Heq; inversions H1; inversions H10.
       apply IHty_trm1; eauto.
       apply IHty_trm2; eauto. apply has_any; assumption.
       apply IHty_trm1; eauto. apply has_any; assumption.
@@ -2508,14 +2516,14 @@ Qed.
 (** * Tight bound completeness *)
 
 Lemma has_member_rcd_typ_sub2_mut:
-  (forall G x T A S U,
-    has_member G x T A S U ->
+  (forall G S x T A V U,
+    has_member G S x T A V U ->
     record_type T ->
-    T = (typ_rcd (dec_typ A S U)) \/ subtyp ty_precise sub_general G T (typ_rcd (dec_typ A S U)))  /\
-  (forall G x T A S U,
-    has_member_rules G x T A S U ->
+    T = (typ_rcd (dec_typ A V U)) \/ subtyp ty_precise sub_general G S T (typ_rcd (dec_typ A V U)))  /\
+  (forall G S x T A V U,
+    has_member_rules G S x T A V U ->
     record_type T ->
-    T = (typ_rcd (dec_typ A S U)) \/ subtyp ty_precise sub_general G T (typ_rcd (dec_typ A S U))).
+    T = (typ_rcd (dec_typ A V U)) \/ subtyp ty_precise sub_general G S T (typ_rcd (dec_typ A V U))).
 Proof.
   apply has_mutind; intros.
   - apply H; eauto.
@@ -2533,8 +2541,8 @@ Proof.
   - destruct H as [ls H]. inversion H.
 Qed.
 
-Lemma wf_stack_val_new_in_G: forall G s x T ds,
-  wf_stack G s ->
+Lemma wf_stack_val_new_in_G: forall G S s x T ds,
+  wf_stack G S s ->
   binds x (val_new T ds) s ->
   binds x (typ_bnd T) G.
 Proof.
@@ -2542,30 +2550,32 @@ Proof.
   assert (exists S, binds x S G) as Bi. {
     eapply stack_binds_to_ctx_binds; eauto.
   }
-  destruct Bi as [S Bi].
-  destruct (corresponding_types Hwf Bi).
-  - destruct H as [? [? [? [Bis' _]]]].
+  destruct Bi as [V Bi].
+  destruct (corresponding_types_ctx Hwf Bi). destruct H as [Hlam | Hnew].
+  - destruct Hlam as [? [? [? [Bis' _]]]].
     unfold binds in Bis'. unfold binds in Bis. rewrite Bis in Bis'. inversion Bis'.
-  - destruct H as [T' [ds' [Bis' [Hty Heq]]]].
+  - destruct Hnew as [T' [ds' [Bis' [Hty Heq]]]].
     unfold binds in Bis'. unfold binds in Bis. rewrite Bis' in Bis. inversions Bis.
     assumption.
+  - destruct H as [V0 [l [Bi' [Hty]]]].
+    unfold binds in Bi'. unfold binds in Bis. rewrite Bi' in Bis. inversion Bis.
 Qed.
 
-(* If G ~ s, s |- x = new(x: T)d, and G |-# x: {A: S..U} then G |-# x.A <: U and G |-# S <: x.A. *)
-Lemma tight_bound_completeness: forall G s x T ds A S U,
-  wf_stack G s ->
+(* If G, S ~ s, s |- x = new(x: T)d, and G, S |-# x: {A: V..U} then G |-# x.A <: U and G, S |-# V <: x.A. *)
+Lemma tight_bound_completeness: forall G S s x T ds A V U,
+  wf_stack G S s ->
   binds x (val_new T ds) s ->
-  ty_trm ty_general sub_tight G (trm_var (avar_f x)) (typ_rcd (dec_typ A S U)) ->
-  subtyp ty_general sub_tight G (typ_sel (avar_f x) A) U /\
-  subtyp ty_general sub_tight G S (typ_sel (avar_f x) A).
+  ty_trm ty_general sub_tight G S (trm_var (avar_f x)) (typ_rcd (dec_typ A V U)) ->
+  subtyp ty_general sub_tight G S (typ_sel (avar_f x) A) U /\
+  subtyp ty_general sub_tight G S V (typ_sel (avar_f x) A).
 Proof.
   introv Hwf Bis Hty.
-  assert (has_member G x (typ_rcd (dec_typ A S U)) A S U) as Hmem. {
+  assert (has_member G S x (typ_rcd (dec_typ A V U)) A V U) as Hmem. {
     apply has_any. assumption. apply has_refl.
   }
   apply has_member_monotonicity with (s:=s) (ds:=ds) (T0:=T) in Hmem.
   destruct Hmem as [T1 [Hmem [Hsub1 Hsub2]]].
-  assert (has_member G x (open_typ x T) A T1 T1) as Hmemx. {
+  assert (has_member G S x (open_typ x T) A T1 T1) as Hmemx. {
     apply has_member_inv in Hmem.
     repeat destruct Hmem as [Hmem|Hmem].
     + inversion Hmem.
@@ -2580,16 +2590,16 @@ Proof.
   assert (record_type (open_typ x T)) as Htypex. {
     apply open_record_type. assumption.
   }
-  assert (open_typ x T = (typ_rcd (dec_typ A T1 T1)) \/ subtyp ty_precise sub_general G (open_typ x T) (typ_rcd (dec_typ A T1 T1))) as Hsub. {
+  assert (open_typ x T = (typ_rcd (dec_typ A T1 T1)) \/ subtyp ty_precise sub_general G S (open_typ x T) (typ_rcd (dec_typ A T1 T1))) as Hsub. {
     destruct has_member_rcd_typ_sub2_mut as [HE _].
     eapply HE; eauto.
   }
-  assert (ty_trm ty_precise sub_general G (trm_var (avar_f x)) (open_typ x T)) as Htypx. {
+  assert (ty_trm ty_precise sub_general G S (trm_var (avar_f x)) (open_typ x T)) as Htypx. {
     eapply ty_rec_elim.
     eapply ty_var.
     eapply wf_stack_val_new_in_G; eauto.
   }
-  assert (ty_trm ty_precise sub_general G (trm_var (avar_f x)) (typ_rcd (dec_typ A T1 T1))) as Htyp. {
+  assert (ty_trm ty_precise sub_general G S (trm_var (avar_f x)) (typ_rcd (dec_typ A T1 T1))) as Htyp. {
     destruct Hsub as [Heq | Hsub].
     - rewrite Heq in Htypx. apply Htypx.
     - eapply ty_sub.
@@ -2605,9 +2615,9 @@ Qed.
 (* ###################################################################### *)
 (** * Misc Inversions *)
 
-Lemma all_intro_inversion: forall G S t U,
-  ty_trm ty_precise sub_general G (trm_val (val_lambda S t)) U ->
-  exists T, U = typ_all S T.
+Lemma all_intro_inversion: forall G S V t U,
+  ty_trm ty_precise sub_general G S (trm_val (val_lambda V t)) U ->
+  exists T, U = typ_all V T.
 Proof.
   intros. dependent induction H.
   - eexists. reflexivity.
